bedrock2/src/bedrock2/Syntax.v
@@ -41,7 +41,8 @@ Module cmd.
   | skip
   | set (lhs : String.string) (rhs : expr)
   | unset (lhs : String.string)
-  | store (_ : access_size) (address : expr) (value : expr)
+  | store (address : expr) (value : expr)
+  | load (lhs : String.string) (address : expr)
   | stackalloc (lhs : String.string) (nbytes : Z) (body : cmd)
   (* { lhs = alloca(nbytes); body; /*allocated memory freed right here*/ } *)
   | cond (condition : expr) (nonzero_branch zero_branch : cmd)
